Addition of basic morphism (without morphism lemmas) between FSets and finite ISets.
(==) is used to denote extensional equality of an ISet (on the left)
and an FSet (on the right). The notation does not make it clear that
the predicate has no symmetry, so a better one might be needed.

finite is an existentially quantified version of (==) (i.e. we define
an ISet as finite iff it is extensionally equal to some FSet).

toFSet takes an ISet and produces an FSet. If its argument is finite,
then the argument and result are extensionally equal.

theories/ISet.ec
@@ -205,26 +205,17 @@ lemma leq_filter: forall (p:'a cpred) X,
   filter p X <= X
 by [].
 
-theory Duni.
-  require import Distr.
-  (** We recall notations from Distr.ec used here:
-      - U denotes a uniformity axiom or lemma,
-      - in_d denotes a support membership test,
-      - d_x is the weight of x in d,
-      - weight_d is the weight of the constantly true predicate in d. *)
-  op duni: 'a set -> 'a distr.
+theory Finite.
+  require        FSet.
 
-  axiom in_duni: forall (x:'a) X, in_supp x (duni X) <=> mem x X.
+  pred (==) (X:'a set) (Y:'a FSet.set) =
+    forall (x:'a), mem x X <=> FSet.mem x Y.
 
-  axiom duniU: forall (X:'a set) x y,
-    mem x X => mem y X =>
-    mu_x (duni X) x = mu_x (duni X) y.
+  pred finite (X:'a set) = exists (X':'a FSet.set), X == X'.
 
-  axiom duni_x_nin: forall (x:'a) X, 
-    !mem x X => mu_x (duni X) x = 0%r.
+  op toFSet: 'a set -> 'a FSet.set.
+  axiom toFSet_cor: forall (X:'a set),
+    finite X => X == toFSet X.
 
-  axiom mu_empty: forall (P:'a cpred), mu (duni empty) P = 0%r.
-
-  axiom weight_duni: forall (X:'a set),
-    weight (duni X) = if X = empty then 0%r else 1%r.
-end Duni.
+  (* We should then show that all set operations correspond as expected *)
+end Finite.
